Done chapter 3

CS_Ch3.thy
@@ -106,4 +106,279 @@ apply(induction e)
 apply(auto)
 done
 
-end
+(* 3.4 is a separate theory, CS_Ch3_Ex4 *)
+
+(* 3.5 *)
+datatype aexp2 = N2 int | V2 vname | Plus2 aexp2 aexp2 | PostIncr2 vname | Div2 aexp2 aexp2
+fun aval2 :: "aexp2 \<Rightarrow> state \<Rightarrow> (val \<times> state) option" where
+"aval2 (N2 i) s = Some (i, s)" |
+"aval2 (V2 x) s = Some (s x, s)" |
+"aval2 (Plus2 a b) s = (case (aval2 a s) of Some (a', s') \<Rightarrow> 
+  (case (aval2 b s') of Some (b', s'') \<Rightarrow> Some (a' + b', s'') | None \<Rightarrow> None) | None \<Rightarrow> None)" |
+"aval2 (PostIncr2 x) s = Some (s x, s(x := (s x) + 1))" |
+"aval2 (Div2 a b) s = (case (aval2 b s) of Some (b', s') \<Rightarrow> (if b' = 0 then None else Some (
+  case (aval2 a s') of Some (a', s'') \<Rightarrow> (a' div b', s''))) | None \<Rightarrow> None)"
+
+lemma "aval2 (Div2 (N2 3) (Plus2 (N2 1) (V2 ''x''))) (\<lambda>x. -1) = None"
+apply(auto)
+done
+
+lemma "case aval2 (Div2 (N2 3) (PostIncr2 ''x'')) (\<lambda>x. 1) of Some (a, b) \<Rightarrow> (a = 3 \<and> b(''x'') = 2) | None \<Rightarrow> False"
+apply(auto)
+done
+
+(* 3.6 *)
+
+datatype lexp = Nl int | Vl vname | Plusl lexp lexp | LET vname lexp lexp
+fun lval :: "lexp \<Rightarrow> state \<Rightarrow> int" where
+"lval (Nl i) s = i" |
+"lval (Vl x) s = s x" |
+"lval (Plusl a b) s = lval a s + lval b s" |
+"lval (LET x val body) s = lval body (s(x := lval val s))"
+
+fun inline :: "lexp \<Rightarrow> aexp" where
+"inline (Nl i) = (N i)" |
+"inline (Vl x) = (V x)" |
+"inline (Plusl a b) = Plus (inline a) (inline b)" |
+"inline (LET x val body) = subst x (inline val) (inline body)"
+
+lemma "lval e s = aval (inline e) s"
+apply(induction e arbitrary: s)
+apply(auto simp add: subst_lemma)
+done
+
+datatype bexp = Bc bool | Not bexp | And bexp bexp | Less aexp aexp
+
+fun bval :: "bexp \<Rightarrow> state \<Rightarrow> bool" where
+"bval (Bc v) s = v" |
+"bval (Not b) s = (\<not> bval b s)" |
+"bval (And b\<^sub>1 b\<^sub>2) s = (bval b\<^sub>1 s \<and> bval b\<^sub>2 s)" |
+"bval (Less a\<^sub>1 a\<^sub>2) s = (aval a\<^sub>1 s < aval a\<^sub>2 s)"
+
+fun not :: "bexp \<Rightarrow> bexp" where
+"not (Bc True) = Bc False" |
+"not (Bc False) = Bc True" |
+"not b = Not b"
+
+fun "and" :: "bexp \<Rightarrow> bexp \<Rightarrow> bexp" where
+"and (Bc True) b = b" |
+"and b (Bc True) = b" |
+"and (Bc False) b = Bc False" |
+"and b (Bc False) = Bc False" |
+"and b\<^sub>1 b\<^sub>2 = And b\<^sub>1 b\<^sub>2"
+
+fun less :: "aexp \<Rightarrow> aexp \<Rightarrow> bexp" where
+"less (aexp.N n\<^sub>1) (aexp.N n\<^sub>2) = Bc (n\<^sub>1 < n\<^sub>2)" |
+"less a\<^sub>1 a\<^sub>2 = Less a\<^sub>1 a\<^sub>2"
+
+fun bsimp :: "bexp \<Rightarrow> bexp" where
+"bsimp (Bc v) = Bc v" |
+"bsimp (Not b) = not (bsimp b)" |
+"bsimp (And b\<^sub>1 b\<^sub>2) = and (bsimp b\<^sub>1) (bsimp b\<^sub>2)" |
+"bsimp (Less a\<^sub>1 a\<^sub>2) = less (asimp a\<^sub>1) (asimp a\<^sub>2)"
+
+(* 3.7 *)
+
+fun Eq :: "aexp \<Rightarrow> aexp \<Rightarrow> bexp" where
+"Eq a b = And (Not (Less a b)) (Not (Less b a))"
+
+lemma "bval (Eq a b) s = (aval a s = aval b s)"
+apply(auto)
+done
+
+fun Le :: "aexp \<Rightarrow> aexp \<Rightarrow> bexp" where
+"Le a b = Not (And (Not (Less a b)) (Not (Eq a b)))"
+
+lemma "bval (Le a b) s = (aval a s \<le> aval b s)"
+apply(auto)
+done
+
+(* 3.8 *)
+datatype ifexp = Bc2 bool | If ifexp ifexp ifexp | Less2 aexp aexp
+
+fun ifval :: "ifexp \<Rightarrow> state \<Rightarrow> bool" where
+"ifval (Bc2 b) s = b" |
+"ifval (If a b c) s = (if ifval a s then ifval b s else ifval c s)" |
+"ifval (Less2 a b) s = (aval a s < aval b s)"
+
+fun b2ifexp :: "bexp \<Rightarrow> ifexp" where
+"b2ifexp (Less a b) = (Less2 a b)" |
+"b2ifexp (Not a) = If (b2ifexp a) (Bc2 False) (Bc2 True)" |
+"b2ifexp (And a b) = If (b2ifexp a) (b2ifexp b) (Bc2 False)" |
+"b2ifexp (Bc b) = Bc2 b"
+
+lemma "bval b s = ifval (b2ifexp b) s"
+apply(induction b)
+apply(auto)
+done
+
+fun if2bexp :: "ifexp \<Rightarrow> bexp" where
+"if2bexp (Bc2 b) = Bc b" |
+"if2bexp (If c t f) = And (Not (And (if2bexp c) (Not (if2bexp t)))) (Not (And (Not (if2bexp c)) (Not (if2bexp f))))" |
+"if2bexp (Less2 a b) = Less a b"
+
+lemma "ifval i s = bval (if2bexp i) s"
+apply(induction i)
+apply(auto)
+done
+
+(* 3.9 *)
+
+datatype pbexp = VAR vname | NOT pbexp | AND pbexp pbexp | OR pbexp pbexp
+
+fun pbval :: "pbexp \<Rightarrow> (vname \<Rightarrow> bool) \<Rightarrow> bool" where
+"pbval (VAR x) s = s x" |
+"pbval (NOT b) s = (\<not> pbval b s)" |
+"pbval (AND b\<^sub>1 b\<^sub>2) s = (pbval b\<^sub>1 s \<and> pbval b\<^sub>2 s)" |
+"pbval (OR b\<^sub>1 b\<^sub>2) s = (pbval b\<^sub>1 s \<or> pbval b\<^sub>2 s)"
+
+fun is_nnf :: "pbexp \<Rightarrow> bool" where
+"is_nnf (VAR x) = True" |
+"is_nnf (NOT (VAR x)) = True" |
+"is_nnf (NOT y) = False" |
+"is_nnf (OR a b) = (is_nnf a \<and> is_nnf b)" |
+"is_nnf (AND a b) = (is_nnf a \<and> is_nnf b)"
+
+fun nnf :: "pbexp \<Rightarrow> pbexp" where
+"nnf (VAR x) = VAR x" |
+"nnf (NOT (VAR x)) = (NOT (VAR x))" |
+"nnf (NOT (AND a b)) = OR (nnf (NOT a)) (nnf (NOT b))" |
+"nnf (NOT (OR a b)) = AND (nnf (NOT a)) (nnf (NOT b))" |
+"nnf (NOT (NOT b)) = nnf b " |
+"nnf (AND a b) = AND (nnf a) (nnf b)" |
+"nnf (OR a b) = OR (nnf a) (nnf b)"
+
+lemma "is_nnf (nnf b)"
+apply(induction b rule: nnf.induct)
+apply(auto)
+done
+
+fun is_dnf :: "pbexp \<Rightarrow> bool" where
+"is_dnf (VAR x) = True" |
+(* since we assume NNF, we don't need to handle NOT *)
+"is_dnf (NOT x) = True" |
+"is_dnf (AND (OR _ _) _) = False" |
+"is_dnf (AND _ (OR _ _)) = False" |
+"is_dnf (AND a b) = (is_dnf a \<and> is_dnf b)" |
+"is_dnf (OR a b) = (is_dnf a \<and> is_dnf b)"
+
+
+fun dnf_of_nnf :: "pbexp \<Rightarrow> pbexp" where
+"dnf_of_nnf (VAR x) = VAR x" |
+"dnf_of_nnf (NOT x) = NOT x" |
+"dnf_of_nnf (OR a b) = OR (dnf_of_nnf a) (dnf_of_nnf b)" |
+"dnf_of_nnf (AND (OR o\<^sub>1 o\<^sub>2) a) = OR (AND o\<^sub>1 a) (AND o\<^sub>2 a)" |
+"dnf_of_nnf (AND a (OR o\<^sub>1 o\<^sub>2)) = OR (AND o\<^sub>1 a) (AND o\<^sub>2 a)" |
+"dnf_of_nnf (AND a b) = AND (dnf_of_nnf a) (dnf_of_nnf b)"
+
+lemma "pbval (dnf_of_nnf b) s = pbval b s"
+apply(induction b rule: dnf_of_nnf.induct)
+apply(auto)
+done
+
+lemma "is_nnf b \<Longrightarrow> is_nnf (dnf_of_nnf b)"
+apply(induction b rule: dnf_of_nnf.induct)
+apply(auto)
+done
+
+datatype instr = LOADI val | LOAD vname | ADD
+type_synonym stack = "val list"
+abbreviation "hd2 xs == hd(tl xs)"
+abbreviation "tl2 xs == tl(tl xs)"
+
+fun exec1 :: "instr \<Rightarrow> state \<Rightarrow> stack \<Rightarrow> stack option" where
+"exec1 (LOADI n) _ stk = Some (n # stk)" |
+"exec1 (LOAD x) s stk = Some ((s x) # stk)" |
+"exec1 ADD _ (h # h2 # rst) = Some ((h2 + h) # rst)" |
+"exec1 ADD _ _ = None"
+
+(* I tried using Option.bind etc but I can't seem to get anything proven when I'm using it.
+   Expanding it manually works, though. Oh well. *)
+fun exec :: "instr list \<Rightarrow> state \<Rightarrow> stack \<Rightarrow> stack option" where
+"exec [] _ stk = Some (stk)" |
+"exec (i # is) s stk = (case (exec1 i s stk) of Some stk' \<Rightarrow> exec is s stk' | None \<Rightarrow> None)"
+
+fun comp :: "aexp \<Rightarrow> instr list" where
+"comp (N n) = [LOADI n]" |
+"comp (V x) = [LOAD x]" |
+"comp (Plus e\<^sub>1 e\<^sub>2) = comp e\<^sub>1 @ comp e\<^sub>2 @ [ADD]"
+
+(* I originally tried to formulate these lemmas like,
+"case (exec is\<^sub>1 s stk) of Some stk' \<Rightarrow> exec (is\<^sub>1 @ is\<^sub>2) s stk = exec is\<^sub>2 s stk' 
+                        | None \<Rightarrow> exec (is\<^sub>1 @ is\<^sub>2) s stk = None"
+but was unable to prove them. *)
+lemma exec_append: "exec is\<^sub>1 s stk = Some stk' \<Longrightarrow> exec (is\<^sub>1 @ is\<^sub>2) s stk = exec is\<^sub>2 s stk'"
+apply(induction is\<^sub>1 arbitrary: stk)
+apply(auto split: option.split)
+done
+
+lemma "exec (comp a) s stk = Some (aval a s # stk)"
+apply(induction a arbitrary: stk)
+apply(auto simp add: exec_append)
+done
+
+(* 3.11 *)
+type_synonym reg = nat
+datatype reginstr = LDI int reg | LD vname reg | ADD reg reg
+
+fun regexec1 :: "reginstr \<Rightarrow> state \<Rightarrow> (reg \<Rightarrow> int) \<Rightarrow> reg \<Rightarrow> int" where
+"regexec1 (LDI v r) s file = file(r := v)" |
+"regexec1 (LD x r) s file = file(r := s x)" |
+"regexec1 (ADD r\<^sub>1 r\<^sub>2) s file = file(r\<^sub>1 := (file r\<^sub>1) + (file r\<^sub>2))"
+
+fun regexec :: "reginstr list \<Rightarrow> state \<Rightarrow> (reg \<Rightarrow> int) \<Rightarrow> reg \<Rightarrow> int" where
+"regexec [] s file = file" |
+"regexec (i # is) s file = regexec is s (regexec1 i s file)"
+
+fun regcomp :: "aexp \<Rightarrow> reg \<Rightarrow> reginstr list" where
+"regcomp (N n) r = [LDI n r]" |
+"regcomp (V x) r = [LD x r]" |
+"regcomp (Plus e\<^sub>1 e\<^sub>2) r = regcomp e\<^sub>1 r @ regcomp e\<^sub>2 (r+1) @ [ADD r (r+1)]"
+
+lemma regexec_append: "regexec (is\<^sub>1 @ is\<^sub>2) s file = regexec is\<^sub>2 s (regexec is\<^sub>1 s file)"
+apply(induction is\<^sub>1 arbitrary: "file")
+apply(auto)
+done
+
+lemma regcomp_dont_touch_small_regs: "q < r \<Longrightarrow> regexec (regcomp a r) s file q = file q"
+apply(induction a arbitrary: r "file")
+apply(auto simp add: regexec_append)
+done
+
+lemma "(regexec (regcomp a r) s file) r = aval a s"
+apply(induction a arbitrary: s r "file")
+apply(auto simp add: regexec_append regcomp_dont_touch_small_regs)
+done
+
+(* 3.12 *)
+datatype instr0 = LDI0 val | LD0 vname | MV0 reg | ADD0 reg
+
+fun exec10 :: "instr0 \<Rightarrow> state \<Rightarrow> (reg \<Rightarrow> int) \<Rightarrow> reg \<Rightarrow> int" where
+"exec10 (LDI0 val) s file = file(0 := val)" |
+"exec10 (LD0 vname) s file = file(0 := s vname)" |
+"exec10 (MV0 reg) s file = file(reg := file 0)" |
+"exec10 (ADD0 reg) s file = file(0 := (file 0) + (file reg))"
+
+fun exec0 :: "instr0 list \<Rightarrow> state \<Rightarrow> (reg \<Rightarrow> int) \<Rightarrow> reg \<Rightarrow> int" where
+"exec0 [] s file = file" |
+"exec0 (i # is) s file = exec0 is s (exec10 i s file)"
+
+fun comp0 :: "aexp \<Rightarrow> reg \<Rightarrow> instr0 list" where
+"comp0 (N n) r = [LDI0 n]" |
+"comp0 (V x) r = [LD0 x]" |
+"comp0 (Plus e\<^sub>1 e\<^sub>2) r = (comp0 e\<^sub>1 (r+1)) @ [MV0 (r+1)] @ (comp0 e\<^sub>2 (r+2)) @ [ADD0 (r+1)]"
+
+lemma exec0_append: "exec0 (is\<^sub>1 @ is\<^sub>2) s file = exec0 is\<^sub>2 s (exec0 is\<^sub>1 s file)"
+apply(induction is\<^sub>1 arbitrary: "file")
+apply(auto)
+done
+
+lemma comp0_register_preservation: "0 \<noteq> q \<Longrightarrow> q < r \<Longrightarrow> exec0 (comp0 a r) s file q = file q"
+apply(induction a arbitrary: r q "file")
+apply(auto simp add: exec0_append)
+done
+
+lemma "exec0 (comp0 a r) s rs 0 = aval a s"
+apply(induction a arbitrary: r s rs)
+apply(auto simp add: exec0_append comp0_register_preservation)
+done
