CS_Ch3_Ex4.thy
@@ -1,0 +1,47 @@
+theory CS_Ch3_Ex4
+imports Main
+begin
+
+type_synonym vname = string
+datatype aexp = N int | V vname | Plus aexp aexp | Times aexp aexp
+type_synonym val = int
+type_synonym state = "vname \<Rightarrow> val"
+
+fun aval :: "aexp \<Rightarrow> state \<Rightarrow> val" where
+"aval (N n) s = n" |
+"aval (V x) s = s x" |
+"aval (Plus a1 a2) s = aval a1 s + aval a2 s" |
+"aval (Times a1 a2) s = aval a1 s * aval a2 s"
+
+fun plus :: "aexp \<Rightarrow> aexp \<Rightarrow> aexp" where
+"plus (N i1) (N i2) = N (i1 + i2)" |
+"plus (N i) a = (if i = 0 then a else Plus (N i) a)" |
+"plus a (N i) = (if i = 0 then a else Plus a (N i))" |
+"plus a1 a2 = Plus a1 a2"
+
+lemma aval_plus: "aval (plus a1 a2) s = aval a1 s + aval a2 s"
+apply(induction a1 a2 rule: plus.induct)
+apply(auto)
+done
+
+fun times :: "aexp \<Rightarrow> aexp \<Rightarrow> aexp" where
+"times (N i1) (N i2) = N (i1 * i2)" |
+"times (N i) a = (if i = 0 then (N 0) else if i = 1 then a else Times (N i) a)" |
+"times a (N i) = (if i = 0 then (N 0) else if i = 1 then a else Times (N i) a)" |
+"times a b = Times a b"
+
+lemma aval_times: "aval (times a1 a2) s = aval a1 s * aval a2 s"
+apply(induction a1 a2 rule: times.induct)
+apply(auto)
+done
+
+fun asimp :: "aexp \<Rightarrow> aexp" where
+"asimp (N n) = N n" |
+"asimp (V x) = V x" |
+"asimp (Plus a1 a2) = plus (asimp a1) (asimp a2)" |
+"asimp (Times a1 a2) = times (asimp a1) (asimp a2)"
+
+lemma "aval (asimp a) s = aval a s"
+apply(induction a)
+apply(auto simp add: aval_plus aval_times)
+done
